libcrux-ml-kem/src/vector/portable.rs
@@ -169,13 +169,16 @@ impl Operations for PortableVector {
         cond_subtract_3329(v)
     }
 
-    #[requires(fstar!(r#"Spec.Utils.is_i16b_array 28296 (impl.f_repr ${v})"#))]
+    #[requires(fstar!(r#"Spec.Utils.is_i16b_array_opaque 28296 (impl.f_repr ${v})"#))]
     fn barrett_reduce(v: Self) -> Self {
+        hax_lib::fstar!(r#"reveal_opaque (`%Spec.Utils.is_i16b_array_opaque) Spec.Utils.is_i16b_array_opaque"#);
         barrett_reduce(v)
     }
 
     #[requires(fstar!(r#"Spec.Utils.is_i16b 1664 $r"#))]
+    #[ensures(|out| fstar!(r#"Spec.Utils.is_i16b_array_opaque 3328 (impl.f_repr $out)"#))]
     fn montgomery_multiply_by_constant(v: Self, r: i16) -> Self {
+        hax_lib::fstar!(r#"reveal_opaque (`%Spec.Utils.is_i16b_array_opaque) Spec.Utils.is_i16b_array_opaque"#);
         montgomery_multiply_by_constant(v, r)
     }
 
@@ -257,9 +260,9 @@ impl Operations for PortableVector {
 
     #[requires(fstar!(r#"Spec.Utils.is_i16b 1664 zeta0 /\ Spec.Utils.is_i16b 1664 zeta1 /\
                        Spec.Utils.is_i16b 1664 zeta2 /\ Spec.Utils.is_i16b 1664 zeta3 /\
-                       Spec.Utils.is_i16b_array 3328 (impl.f_repr ${lhs}) /\
-                       Spec.Utils.is_i16b_array 3328 (impl.f_repr ${rhs})"#))]
-    #[ensures(|out| fstar!(r#"Spec.Utils.is_i16b_array 3328 (impl.f_repr $out)"#))]
+                       Spec.Utils.is_i16b_array_opaque 3328 (impl.f_repr ${lhs}) /\
+                       Spec.Utils.is_i16b_array_opaque 3328 (impl.f_repr ${rhs})"#))]
+    #[ensures(|out| fstar!(r#"Spec.Utils.is_i16b_array_opaque 3328 (impl.f_repr $out)"#))]
     fn ntt_multiply(
         lhs: &Self,
         rhs: &Self,
@@ -268,6 +271,7 @@ impl Operations for PortableVector {
         zeta2: i16,
         zeta3: i16,
     ) -> Self {
+        hax_lib::fstar!(r#"reveal_opaque (`%Spec.Utils.is_i16b_array_opaque) Spec.Utils.is_i16b_array_opaque"#);
         ntt_multiply(lhs, rhs, zeta0, zeta1, zeta2, zeta3)
     }
 
